src/cbor/raw/pulse/CBOR.Pulse.Raw.Util.fst
@@ -1,0 +1,22 @@
+module CBOR.Pulse.Raw.Util
+open Pulse.Lib.Pervasives
+
+let perm_mul (p1 p2: perm) : Tot perm = p1 *. p2
+
+#reset-options "--smtencoding.elim_box true --smtencoding.l_arith_repr native --smtencoding.nl_arith_repr native"
+
+let perm_mul_assoc
+  (p1 p2 p3: perm)
+: Lemma
+  (ensures (p1 `perm_mul` (p2 `perm_mul` p3) == (p1 `perm_mul` p2) `perm_mul` p3))
+  [SMTPatOr [
+    [SMTPat (p1 `perm_mul` (p2 `perm_mul` p3))];
+    [SMTPat ((p1 `perm_mul` p2) `perm_mul` p3)];
+  ]]
+= ()
+
+let perm_1_l
+  (p: perm)
+: Lemma
+  (1.0R `perm_mul` p == p)
+= ()
